examples/scalaEquivalenceBenchmarkExamples/noHelp/whacAFun6.dfy
@@ -9,14 +9,6 @@ function rep2<A>(n: int, f: A -> A, a: A): A
   repeat2(n, f)(a)
 }
 
-lemma equivalenceRep<A>(n: int, f: A -> A, a: A)
-  requires n >= 0
-  ensures rep1(n, f, a) == rep2(n, f, a)
-{
-  equivalenceRepeat12(n, f, a);
-}
-
-// Said to be non-equivalent, even though they are :(
 function repeat1<A>(n: int, f: A -> A): A -> A
   requires (n >= 0)
   decreases(n) {
@@ -30,13 +22,4 @@ function repeat2<A>(n: int, f: A -> A): A -> A
   decreases(n) {
   if (n == 0) then a => a
   else a => repeat2(n - 1, f)(f(a))
-}
-
-lemma equivalenceRepeat12<A>(n: int, f: A -> A, a: A)
-  requires n >= 0
-  ensures repeat1(n, f)(a) == repeat2(n, f)(a)
-{
-  if n > 0 {
-    equivalenceRepeat12(n - 1, f, f(a));
-  }
 }
