examples/scalaEquivalenceBenchmarkExamples/fullHelp/whacAFun6.dfy
@@ -1,0 +1,41 @@
+// Times out
+function rep1<A>(n: int, f: A -> A, a: A): A
+  requires (n >= 0) {
+  repeat1(n, f)(a)
+}
+
+function rep2<A>(n: int, f: A -> A, a: A): A
+  requires (n >= 0) {
+  repeat2(n, f)(a)
+}
+
+lemma equivalenceRep<A>(n: int, f: A -> A, a: A)
+  requires n >= 0
+  ensures rep1(n, f, a) == rep2(n, f, a)
+{
+  equivalenceRepeat12(n, f, a);
+}
+
+function repeat1<A>(n: int, f: A -> A): A -> A
+  requires (n >= 0)
+  decreases(n) {
+  a =>
+    if (n == 0) then a
+    else repeat1(n - 1, f)(f(a))
+}
+
+function repeat2<A>(n: int, f: A -> A): A -> A
+  requires (n >= 0)
+  decreases(n) {
+  if (n == 0) then a => a
+  else a => repeat2(n - 1, f)(f(a))
+}
+
+lemma equivalenceRepeat12<A>(n: int, f: A -> A, a: A)
+  requires n >= 0
+  ensures repeat1(n, f)(a) == repeat2(n, f)(a)
+{
+  if n > 0 {
+    equivalenceRepeat12(n - 1, f, f(a));
+  }
+}
