src/test/output/whacAFun6.dfy
@@ -1,0 +1,29 @@
+function rep1<A>(n: int, f: A -> A, a: A): A
+requires (n >= 0)
+{repeat1(n, f)(a)}
+
+function rep2<A>(n: int, f: A -> A, a: A): A
+requires (n >= 0)
+{repeat2(n, f)(a)}
+
+function repeat2<A>(n: int, f: A -> A): A -> A
+requires (n >= 0)
+decreases (n)
+{if (n == 0) then (a) => a else (a) => repeat2((n - 1), f)(f(a))}
+
+function repeat1<A>(n: int, f: A -> A): A -> A
+requires (n >= 0)
+decreases (n)
+{(a) => if (n == 0) then a else repeat1((n - 1), f)(f(a))}
+
+lemma rep1_rep2_Equivalence<A>(n: int, f: A -> A, a: A)
+requires (n >= 0)
+ensures (rep1(n, f, a) == rep2(n, f, a))
+{{repeat1_repeat2_Equivalence(n, f, a);}}
+
+lemma repeat1_repeat2_Equivalence<A>(n: int, f: A -> A, a: A)
+requires (n >= 0)
+decreases (n)
+ensures (repeat1(n, f)(a) == repeat2(n, f)(a))
+{{if (n == 0){}else {repeat1_repeat2_Equivalence((n - 1), f, f(a));}}}
+
